messageInvariantPrototypes/paxos/centralized_monotonic/applicationProof.dfy
@@ -1,0 +1,549 @@
+include "spec.dfy"
+
+module PaxosProof {
+  
+import opened Types
+import opened UtilitiesLibrary
+import opened System
+import opened Obligations
+
+
+ghost predicate OneValuePerBallot(c: Constants, v: Variables)
+  requires v.WF(c)
+{
+  && OneValuePerBallotAcceptors(c, v)
+  && OneValuePerBallotLearners(c, v)
+  && OneValuePerBallotAcceptorsAndLearners(c, v)
+  && OneValuePerBallotLeaderAndLearners(c, v)
+  && OneValuePerBallotLeaderAndAcceptors(c, v)
+}
+
+// Acceptors only have one value for each ballot
+ghost predicate OneValuePerBallotAcceptors(c: Constants, v: Variables)
+  requires v.WF(c)
+{
+  forall a1, a2 |
+    && c.ValidAcceptorIdx(a1)
+    && c.ValidAcceptorIdx(a2)
+    && v.acceptors[a1].Last().acceptedVB.Some?
+    && v.acceptors[a2].Last().acceptedVB.Some?
+    && v.acceptors[a1].Last().acceptedVB.value.b 
+        == v.acceptors[a2].Last().acceptedVB.value.b 
+  ::
+    v.acceptors[a1].Last().acceptedVB.value.v
+        == v.acceptors[a2].Last().acceptedVB.value.v
+}
+
+// Learners only have one value for each ballot
+ghost predicate OneValuePerBallotLearners(c: Constants, v: Variables)
+  requires v.WF(c)
+{
+  forall l1, l2, vb1, vb2 |
+    && c.ValidLearnerIdx(l1)
+    && c.ValidLearnerIdx(l2)
+    && vb1 in v.learners[l1].Last().receivedAccepts
+    && vb2 in v.learners[l1].Last().receivedAccepts
+    && vb1.b == vb2.b
+  ::
+    vb1.v == vb2.v
+}
+
+// Learners and Acceptors only have one value for each ballot
+ghost predicate OneValuePerBallotAcceptorsAndLearners(c: Constants, v: Variables)
+  requires v.WF(c)
+{
+  forall a, l, vb1, vb2 |
+    && c.ValidAcceptorIdx(a)
+    && c.ValidLearnerIdx(l)
+    && v.acceptors[a].HasAccepted(vb1)
+    && vb2 in v.learners[l].Last().receivedAccepts
+    && vb1.b == vb2.b
+  ::
+    vb1.v == vb2.v
+}
+
+// Leaders and Learners only have one value for each ballot
+ghost predicate OneValuePerBallotLeaderAndLearners(c: Constants, v: Variables)
+  requires v.WF(c)
+{
+  forall ldr, lnr, acceptedVal |
+    && c.ValidLeaderIdx(ldr)
+    && c.ValidLearnerIdx(lnr)
+    && v.LeaderCanPropose(c, ldr)
+    && VB(acceptedVal, ldr) in v.learners[lnr].Last().receivedAccepts
+  ::
+    acceptedVal == v.leaders[ldr].Last().value
+}
+
+// Leaders and Acceptors only have one value for each ballot
+ghost predicate OneValuePerBallotLeaderAndAcceptors(c: Constants, v: Variables)
+  requires v.WF(c)
+{
+  forall ldr, acc, acceptedVal |
+    && c.ValidLeaderIdx(ldr)
+    && c.ValidAcceptorIdx(acc)
+    && v.LeaderCanPropose(c, ldr)
+    && v.acceptors[acc].HasAccepted(VB(acceptedVal, ldr))
+  ::
+    acceptedVal == v.leaders[ldr].Last().value
+}
+
+// Learner's receivedAccepts contain valid acceptor ids
+ghost predicate LearnerValidReceivedAccepts(c: Constants, v: Variables)
+  requires v.WF(c)
+{
+  forall lnr:LearnerId, vb:ValBal, e:AcceptorId |
+    && c.ValidLearnerIdx(lnr)
+    && vb in v.learners[lnr].Last().receivedAccepts
+    && e in v.learners[lnr].Last().receivedAccepts[vb]
+  ::
+    c.ValidAcceptorIdx(e)
+}
+
+// Learner's receivedAccepts contain valid leader ballots
+ghost predicate LearnerValidReceivedAcceptsKeys(c: Constants, v: Variables)
+  requires v.WF(c)
+{
+  forall lnr:LearnerId, vb:ValBal |
+    && c.ValidLearnerIdx(lnr)
+    && vb in v.learners[lnr].Last().receivedAccepts
+  ::
+    c.ValidLeaderIdx(vb.b)
+}
+
+ghost predicate LearnerReceivedAcceptImpliesProposed(c: Constants, v: Variables) 
+  requires v.WF(c)
+  requires LearnerValidReceivedAcceptsKeys(c, v)
+{
+  forall lnr:LearnerId, vb:ValBal |
+    && c.ValidLearnerIdx(lnr)
+    && vb in v.learners[lnr].Last().receivedAccepts
+  ::
+    && v.LeaderCanPropose(c, vb.b)
+    && v.leaders[vb.b].Last().value == vb.v
+}
+
+// Learner's learned value must be backed by a quorum of accepts
+ghost predicate LearnedImpliesQuorumOfAccepts(c: Constants, v: Variables)
+  requires v.WF(c)
+{
+  forall lnr:LearnerId, val:Value |
+    && c.ValidLearnerIdx(lnr)
+    && v.learners[lnr].HasLearnedValue(val)
+  ::
+    exists b: LeaderId ::
+      && var vb := VB(val, b);
+      && ChosenAtLearner(c, v, vb, lnr)
+}
+
+// Each entry in a learner's receivedAccepts implies that an acceptor accepted it
+ghost predicate LearnerReceivedAcceptImpliesAccepted(c: Constants, v: Variables)
+  requires v.WF(c)
+{
+  forall lnr:LearnerId, vb:ValBal, acc:AcceptorId |
+    && c.ValidLearnerIdx(lnr)
+    && c.ValidAcceptorIdx(acc)
+    && vb in v.learners[lnr].Last().receivedAccepts
+    && acc in v.learners[lnr].Last().receivedAccepts[vb]
+  ::
+    v.acceptors[acc].HasAcceptedAtLeastBal(vb.b) 
+}
+
+// Acceptor's fields all host valid leader ballots
+ghost predicate AcceptorValidPromisedAndAccepted(c: Constants, v:Variables) 
+  requires v.WF(c)
+{
+  forall acc: AcceptorId | c.ValidAcceptorIdx(acc)
+  ::
+    && (v.acceptors[acc].Last().pendingPrepare.Some? 
+        ==> c.ValidLeaderIdx(v.acceptors[acc].Last().pendingPrepare.value.bal))
+    && (v.acceptors[acc].Last().promised.Some? 
+        ==> c.ValidLeaderIdx(v.acceptors[acc].Last().promised.value))
+    && (v.acceptors[acc].Last().acceptedVB.Some? 
+        ==> c.ValidLeaderIdx(v.acceptors[acc].Last().acceptedVB.value.b))
+}
+
+// If an acceptor has accepted vb, then it must have promised a ballot >= vb.b
+ghost predicate AcceptorPromisedLargerThanAccepted(c: Constants, v: Variables) 
+  requires v.WF(c)
+{
+  forall acc | 
+    && c.ValidAcceptorIdx(acc) 
+    && v.acceptors[acc].Last().acceptedVB.Some?
+  :: 
+    && v.acceptors[acc].Last().promised.Some?
+    && v.acceptors[acc].Last().acceptedVB.value.b <= v.acceptors[acc].Last().promised.value
+}
+
+ghost predicate AcceptorAcceptedImpliesProposed(c: Constants, v: Variables) 
+  requires v.WF(c)
+  requires AcceptorValidPromisedAndAccepted(c, v)
+{
+  forall acc:AcceptorId |
+    && c.ValidAcceptorIdx(acc)
+    && v.acceptors[acc].Last().acceptedVB.Some?
+  ::
+    var vb := v.acceptors[acc].Last().acceptedVB.value;
+    && v.LeaderCanPropose(c, vb.b)
+    && v.leaders[vb.b].Last().value == vb.v
+}
+
+ghost predicate LeaderValidReceivedPromises(c: Constants, v: Variables)
+  requires v.WF(c)
+{
+  forall ldr, acc |
+    && c.ValidLeaderIdx(ldr)
+    && acc in v.leaders[ldr].Last().receivedPromises
+  ::
+    c.ValidAcceptorIdx(acc)
+}
+
+// For all leaders, its highestHeardBallot is upper bounded by its own ballot
+ghost predicate LeaderHighestHeardUpperBound(c: Constants, v: Variables) 
+  requires v.WF(c)
+{
+  forall ldr:LeaderId | 
+    && c.ValidLeaderIdx(ldr)
+    && v.leaders[ldr].Last().highestHeardBallot.Some?
+  :: 
+    v.leaders[ldr].Last().highestHeardBallot.value < ldr
+}
+
+// If a leader has a highestHeardBallot B, then its value has been proposed by the leader 
+// with ballot B
+ghost predicate LeaderHearedImpliesProposed(c: Constants, v: Variables) 
+  requires v.WF(c)
+{
+  forall ldr:LeaderId | 
+    && c.ValidLeaderIdx(ldr)
+    && v.leaders[ldr].Last().highestHeardBallot.Some?
+  ::
+    // note that once a leader CanPropose(), its value does not change
+    var b := v.leaders[ldr].Last().highestHeardBallot.value;
+    && c.ValidLeaderIdx(b)
+    && v.LeaderCanPropose(c, b)
+    && v.leaders[b].Last().value == v.leaders[ldr].Last().value
+}
+
+// For all ldr, acc such that acc in ldr.receivedPromises, acc's current promise
+// must be >= ldr's ballot
+ghost predicate LeaderReceivedPromisesImpliesAcceptorState(c: Constants, v: Variables)
+  requires v.WF(c)
+{
+  forall ldr:LeaderId, acc:AcceptorId |
+    && c.ValidLeaderIdx(ldr)
+    && c.ValidAcceptorIdx(acc)
+    && acc in v.leaders[ldr].Last().receivedPromises
+  ::
+    v.acceptors[acc].HasPromisedAtLeast(ldr)
+}
+
+// If an acceptor A accepted ballot b, and a leader L has highestHeardBallot < b, then 
+// L cannot have received a promise from A
+ghost predicate LeaderNotHeardImpliesNotPromised(c: Constants, v: Variables)
+  requires v.WF(c)
+{
+  forall ldr:LeaderId, acc:AcceptorId, b:LeaderId |
+    && c.ValidLeaderIdx(ldr)
+    && c.ValidAcceptorIdx(acc)
+    && b < ldr
+    && v.acceptors[acc].HasAcceptedAtLeastBal(b)
+    // Tony: Did not have this line below, which this invariant false
+    && v.acceptors[acc].HasAcceptedAtMostBal(ldr)
+    && v.leaders[ldr].HeardAtMost(b)
+  ::
+    && acc !in v.leaders[ldr].Last().receivedPromises
+}
+
+
+// For any leader L, if an acceptor A is in L.promises, then A cannot have accepted any
+// ballot b such that L.highestHeard < b < L
+ghost predicate LeaderHighestHeardToPromisedRangeHasNoAccepts(c: Constants, v: Variables)
+  requires v.WF(c)
+{
+  forall ldr, acc, lnr, vb:ValBal | 
+    && c.ValidLeaderIdx(ldr)
+    && c.ValidAcceptorIdx(acc)
+    && c.ValidLearnerIdx(lnr)
+    && vb in v.learners[lnr].Last().receivedAccepts
+    && vb.b < ldr
+    && v.leaders[ldr].HeardAtMost(vb.b)
+    && acc in v.leaders[ldr].Last().receivedPromises
+  ::
+    acc !in v.learners[lnr].Last().receivedAccepts[vb]
+}
+
+ghost predicate ChosenValImpliesAcceptorOnlyAcceptsVal(c: Constants, v: Variables) 
+  requires v.WF(c)
+{
+  forall vb, acc:AcceptorId | 
+    && Chosen(c, v, vb)
+    && c.ValidAcceptorIdx(acc)
+    && v.acceptors[acc].Last().acceptedVB.Some?
+    && v.acceptors[acc].Last().acceptedVB.value.b >= vb.b
+  ::
+     v.acceptors[acc].Last().acceptedVB.value.v == vb.v
+}
+
+// If vb is chosen, then for all leaders > vb.b and ready to propose, they must have highest 
+// heard >= b
+ghost predicate ChosenImpliesProposingLeaderHearsChosenBallot(c: Constants, v: Variables)
+  requires v.WF(c)
+{
+  forall vb, ldrBal:LeaderId | 
+    && Chosen(c, v, vb)
+    && c.ValidLeaderIdx(ldrBal)
+    && vb.b < ldrBal
+    && v.LeaderCanPropose(c, ldrBal)
+  ::
+    v.leaders[ldrBal].HeardAtLeast(vb.b)
+}
+
+// If vb is chosen, then for all leaders has a highest heard >= vb.b, the value must be vb.v
+ghost predicate ChosenValImpliesLeaderOnlyHearsVal(c: Constants, v: Variables) 
+  requires v.WF(c)
+{
+  forall vb, ldrBal:LeaderId | 
+    && Chosen(c, v, vb)
+    && c.ValidLeaderIdx(ldrBal)
+    && v.leaders[ldrBal].Last().highestHeardBallot.Some?
+    && v.leaders[ldrBal].Last().highestHeardBallot.value >= vb.b
+  ::
+    v.leaders[ldrBal].Last().value == vb.v
+}
+
+// Application bundle
+ghost predicate ApplicationInv(c: Constants, v: Variables)
+  requires v.WF(c)
+{
+  && OneValuePerBallot(c, v)
+  && LearnerValidReceivedAccepts(c, v)
+  && LearnerValidReceivedAcceptsKeys(c, v)
+  && LearnedImpliesQuorumOfAccepts(c, v)
+  && LearnerReceivedAcceptImpliesProposed(c, v)
+  && LearnerReceivedAcceptImpliesAccepted(c, v)
+  && AcceptorValidPromisedAndAccepted(c, v)
+  && AcceptorPromisedLargerThanAccepted(c, v)
+  && AcceptorAcceptedImpliesProposed(c, v)
+  && LeaderValidReceivedPromises(c, v)
+  && LeaderHighestHeardUpperBound(c, v)
+  && LeaderHearedImpliesProposed(c, v)
+  && LeaderReceivedPromisesImpliesAcceptorState(c, v)
+  && LeaderNotHeardImpliesNotPromised(c, v)
+  && LeaderHighestHeardToPromisedRangeHasNoAccepts(c, v)
+  && ChosenValImpliesAcceptorOnlyAcceptsVal(c, v)
+  && ChosenImpliesProposingLeaderHearsChosenBallot(c, v)
+  && ChosenValImpliesLeaderOnlyHearsVal(c, v)
+}
+
+ghost predicate Inv(c: Constants, v: Variables)
+{
+  && v.WF(c)
+  && ApplicationInv(c, v)
+  && Agreement(c, v)
+}
+
+
+/***************************************************************************************
+*                                Top-level Obligations                                 *
+***************************************************************************************/
+
+
+lemma InvImpliesSafety(c: Constants, v: Variables)
+  requires Inv(c, v)
+  ensures Agreement(c, v)
+{}
+
+lemma InitImpliesInv(c: Constants, v: Variables)
+  requires Init(c, v)
+  ensures Inv(c, v)
+{}
+
+lemma InvInductive(c: Constants, v: Variables, v': Variables)
+  requires Inv(c, v)
+  requires Next(c, v, v')
+  ensures Inv(c, v')
+{
+  assume false;
+  assert AtMostOneChosenVal(c, v');  // this should be implied by invariants
+  AtMostOneChosenImpliesSafety(c, v');
+}
+
+
+/***************************************************************************************
+*                                 InvNext Proofs                                       *
+***************************************************************************************/
+
+// Bundle for simple-to-prove invariants
+lemma InvInductiveHelper(c: Constants, v: Variables, v': Variables)
+  requires Inv(c, v)
+  requires Next(c, v, v')
+  ensures LearnerValidReceivedAccepts(c, v')
+  ensures LearnerValidReceivedAcceptsKeys(c, v')
+  ensures LearnerReceivedAcceptImpliesProposed(c, v')
+  ensures LearnerReceivedAcceptImpliesAccepted(c, v')
+  ensures AcceptorValidPromisedAndAccepted(c, v')
+  ensures AcceptorAcceptedImpliesProposed(c, v')
+  ensures AcceptorPromisedLargerThanAccepted(c, v')
+  ensures LeaderValidReceivedPromises(c, v')
+  ensures LeaderHighestHeardUpperBound(c, v')
+  ensures LeaderHearedImpliesProposed(c, v')
+  ensures LeaderReceivedPromisesImpliesAcceptorState(c, v')
+{}
+
+lemma {:timeLimitMultiplier 2} InvNextOneValuePerBallot(c: Constants, v: Variables, v': Variables)
+  requires v.WF(c)
+  requires OneValuePerBallot(c, v)
+  requires LearnerValidReceivedAcceptsKeys(c, v)  // prereq for LearnerReceivedAcceptImpliesProposed
+  requires AcceptorValidPromisedAndAccepted(c, v) // prereq for AcceptorAcceptedImpliesProposed
+  requires LearnerReceivedAcceptImpliesProposed(c, v)
+  requires AcceptorAcceptedImpliesProposed(c, v)
+  requires Next(c, v, v')
+  ensures OneValuePerBallot(c, v')
+{}
+
+lemma InvNextLearnedImpliesQuorumOfAccepts(c: Constants, v: Variables, v': Variables)
+  requires v.WF(c)
+  requires LearnerValidReceivedAccepts(c, v)
+  requires LearnedImpliesQuorumOfAccepts(c, v)
+  requires Next(c, v, v')
+  ensures LearnedImpliesQuorumOfAccepts(c, v')
+{
+  forall lnr:LearnerId, val:Value |
+    c.ValidLearnerIdx(lnr) && v'.learners[lnr].HasLearnedValue(val)
+  ensures
+    exists b: LeaderId ::
+      && var vb := VB(val, b);
+      && ChosenAtLearner(c, v', vb, lnr)
+  {
+    var sysStep :| NextStep(c, v, v', sysStep);
+    if sysStep.P2bStep? && sysStep.learner == lnr {
+      assert v.learners[lnr].HasLearnedValue(val);  // trigger
+    } else if sysStep.LearnerInternalStep? && sysStep.learner == lnr {
+      var step :| LearnerHost.NextStep(c.learnerConstants[lnr], v.learners[lnr], v'.learners[lnr], step, LearnerHost.InternalLbl());
+      if step.StutterStep? {
+        assert v.learners[lnr].HasLearnedValue(val);  // trigger
+      }
+    }
+  }
+}
+
+/***************************************************************************************
+*                            Helper Definitions and Lemmas                             *
+***************************************************************************************/
+
+ghost predicate IsAcceptorQuorum(c: Constants, quorum: set<AcceptorId>) {
+  && |quorum| >= c.f+1
+  && (forall id | id in quorum :: c.ValidAcceptorIdx(id))
+}
+
+// A learner holds an accept quorum for vb
+ghost predicate Chosen(c: Constants, v: Variables, vb: ValBal) 
+  requires v.WF(c)
+{
+  exists lnr:LearnerId :: ChosenAtLearner(c, v, vb, lnr)
+}
+
+// Learner lnr witnessed a vb being chosen
+ghost predicate ChosenAtLearner(c: Constants, v: Variables, vb: ValBal, lnr:LearnerId) 
+  requires v.WF(c)
+{
+  && c.ValidLearnerIdx(lnr)
+  && vb in v.learners[lnr].Last().receivedAccepts
+  && IsAcceptorQuorum(c, v.learners[lnr].Last().receivedAccepts[vb])
+}
+
+// At most one value can become Chosen
+ghost predicate AtMostOneChosenVal(c: Constants, v: Variables) 
+  requires v.WF(c)
+{
+  forall vb1, vb2 | Chosen(c, v, vb1) && Chosen(c, v, vb2) 
+  :: vb1.v == vb2.v
+}
+
+
+//// Helper Lemmas ////
+
+// A value being learned implies it was chosen at some ballot, and skolemize this ballot
+lemma LearnedImpliesChosen(c: Constants, v: Variables, lnr: LearnerId, val: Value) returns (vb: ValBal)
+  requires v.WF(c)
+  requires c.ValidLearnerIdx(lnr)
+  requires v.learners[lnr].HasLearnedValue(val)
+  requires LearnedImpliesQuorumOfAccepts(c, v)
+  ensures vb.v == val
+  ensures Chosen(c, v, vb)
+{
+  // Witness, given by LearnedImpliesQuorumOfAccepts
+  var bal :| ChosenAtLearner(c, v, VB(val, bal), lnr);
+  return VB(val, bal);
+}
+
+// If only one value can be chosen, then Agreement must be satisfied
+lemma AtMostOneChosenImpliesSafety(c: Constants, v: Variables)
+  requires v.WF(c)
+  requires AtMostOneChosenVal(c, v)
+  requires LearnedImpliesQuorumOfAccepts(c, v)
+  ensures Agreement(c, v)
+{
+  // Proof by contradiction
+  if !Agreement(c, v) {
+    var l1, l2 :| 
+        && c.ValidLearnerIdx(l1)
+        && c.ValidLearnerIdx(l2)
+        && v.learners[l1].HasLearnedSome()
+        && v.learners[l2].HasLearnedSome()
+        && v.learners[l1].GetLearnedValue() != v.learners[l2].GetLearnedValue()
+    ;
+    var vb1 := LearnedImpliesChosen(c, v, l1, v.learners[l1].Last().learned.value);
+    var vb2 := LearnedImpliesChosen(c, v, l2, v.learners[l2].Last().learned.value);
+    assert false;
+  }
+}
+
+// Lemma: The only system step in which a new vb can be chosen is a P2bStep 
+lemma NewChosenOnlyInP2bStep(c: Constants, v: Variables, v': Variables, sysStep: Step) 
+  requires v.WF(c)
+  requires Next(c, v, v')
+  requires NextStep(c, v, v', sysStep)
+  requires !sysStep.P2bStep?
+  ensures forall vb | Chosen(c, v', vb) :: Chosen(c, v, vb)
+{
+  forall vb | Chosen(c, v', vb)
+  ensures Chosen(c, v, vb)
+  {
+    var lnr:LearnerId :| ChosenAtLearner(c, v', vb, lnr);   // witness
+    assert ChosenAtLearner(c, v, vb, lnr);                  // trigger
+  }
+}
+
+// Suppose vb is chosen. Return the quorum of acceptors supporting the chosen vb
+lemma SupportingAcceptorsForChosen(c: Constants, v: Variables, vb: ValBal)
+returns (supportingAccs: set<AcceptorId>)
+  requires v.WF(c)
+  requires Chosen(c, v, vb)
+  requires LearnerReceivedAcceptImpliesAccepted(c, v)
+  ensures |supportingAccs| >= c.f+1
+  ensures forall a | a in supportingAccs :: 
+    && c.ValidAcceptorIdx(a)
+    && v.acceptors[a].HasAcceptedAtLeastBal(vb.b)
+  ensures exists lnr :: 
+    && c.ValidLearnerIdx(lnr)
+    && vb in v.learners[lnr].Last().receivedAccepts
+    && supportingAccs <= v.learners[lnr].Last().receivedAccepts[vb]
+{
+  var lnr: LearnerId :| ChosenAtLearner(c, v, vb, lnr);  // skolemize!
+  supportingAccs := v.learners[lnr].Last().receivedAccepts[vb];
+  return supportingAccs;
+}
+
+lemma GetAcceptorSet(c: Constants, v: Variables)
+returns (accSet: set<AcceptorId>)
+  requires v.WF(c)
+  ensures forall a :: c.ValidAcceptorIdx(a) <==> a in accSet
+  ensures |accSet| == 2 * c.f + 1
+{
+  accSet := set a |  0 <= a < |c.acceptorConstants|;
+  SetComprehensionSize(|c.acceptorConstants|);
+}
+
+} // end module PaxosProof
